case_study/RiscvPmp/BlockVer/Spec.v
@@ -776,20 +776,20 @@ Module RiscvPmpSpecVerif.
   Proof.
     intros.
     destruct f; try discriminate H; eexists.
-    - apply (valid_contract _ H valid_execute_rX).
-    - apply (valid_contract _ H valid_execute_wX).
-    - apply (valid_contract _ H valid_execute_tick_pc).
-    - apply (valid_contract_debug _ H valid_contract_within_phys_mem).
-    - apply (valid_contract _ H valid_mem_read).
-    - apply (valid_contract _ H valid_checked_mem_read).
-    - apply (valid_contract _ H valid_checked_mem_write).
-    - apply (valid_contract _ H valid_pmp_mem_read).
-    - apply (valid_contract _ H valid_pmp_mem_write).
-    - apply (valid_contract_with_fuel_debug _ _ H valid_pmpCheck).
-    - apply (valid_contract_debug _ H valid_pmpMatchAddr).
-    - apply (valid_contract _ H valid_mem_write_value).
-    - apply (valid_contract _ H valid_execute_fetch).
-    - apply (valid_contract_debug _ H valid_contract_execute_EBREAK).
+    - refine (valid_contract _ H valid_execute_rX).
+    - refine (valid_contract _ H valid_execute_wX).
+    - refine (valid_contract _ H valid_execute_tick_pc).
+    - refine (valid_contract_debug _ H valid_contract_within_phys_mem).
+    - refine (valid_contract _ H valid_mem_read).
+    - refine (valid_contract _ H valid_checked_mem_read).
+    - refine (valid_contract _ H valid_checked_mem_write).
+    - refine (valid_contract _ H valid_pmp_mem_read).
+    - refine (valid_contract _ H valid_pmp_mem_write).
+    - refine (valid_contract_with_fuel_debug _ _ H valid_pmpCheck).
+    - refine (valid_contract_debug _ H valid_pmpMatchAddr).
+    - refine (valid_contract _ H valid_mem_write_value).
+    - refine (valid_contract _ H valid_execute_fetch).
+    - refine (valid_contract_debug _ H valid_contract_execute_EBREAK).
   Qed.
 End RiscvPmpSpecVerif.
 
